---
title: Question-31
pagetitle: Question-31
order: 31
categories: [algebra, aptitude]
---

If two distinct non-zero real variables $x$ and $y$ are such that $(x+y)$ is proportional to $(x-y)$ then the value of $\cfrac{x^2+y^2}{x^2-y^2}$ is

- [ ] depends on $xy$
- [ ] depends only on $x$ and not on $y$
- [ ] depends only on $y$ and not on $x$
- [ ] is a constant

::: {.callout-note title="Answer" collapse=true}

- [ ] depends on $xy$
- [ ] depends only on $x$ and not on $y$
- [ ] depends only on $y$ and not on $x$
- [x] is a constant

:::

::: {.callout-note title="Soluton" collapse=true}

Let $\displaystyle x+y=k( x-y)$, with $\displaystyle x,y\neq 0$ and $\displaystyle x,y\in \mathbb{R}$, then:

$$
\begin{aligned}
x+y & =k( x-y)\\
 & \\
( 1-k) x & =-( 1+k) y\\
 & \\
\frac{x}{y} & =\frac{k+1}{k-1}
\end{aligned}
$$

provided $\displaystyle k\neq 1$. $\displaystyle k$ can't be equal to $\displaystyle 1$ since that would lead to $\displaystyle y=0$, which is not possible as per the constraints in the question. We now see that $\displaystyle x$ is proportional to $\displaystyle y$ with some other proportionality constant. Now:

$$
\begin{aligned}
\frac{x^{2} +y^{2}}{x^{2} -y^{2}} & =\frac{\frac{x^{2}}{y^{2}} +1}{\frac{x^{2}}{y^{2}} -1}\\
 & \\
 & =\frac{k^{2} +1}{2k}
\end{aligned}
$$

We see that $\displaystyle \frac{x^{2} +y^{2}}{x^{2} -y^{2}}$ is a constant.

:::


